revising Pulse.Lib.HashTable

pulse/share/steel/examples/pulse/lib/Pulse.Lib.HashTable.fst
@@ -10,25 +10,26 @@ module PHT = Pulse.Lib.HashTable.Spec
 
 #push-options "--using_facts_from '* -FStar.Tactics -FStar.Reflection'"
 
-let models (s:pht_sig_us) (ht:ht_t s) (pht:pht_t (s_to_ps s)) : vprop
-= A.pts_to ht.contents pht.repr **
+let models #kt #vt (ht:ht_t kt vt) (pht:pht_t kt vt) : vprop
+= A.pts_to ht.contents pht.repr.seq **
   pure (
-    SZ.v ht.sz == pht.sz /\
+    SZ.v ht.sz == pht.repr.sz /\
+    pht.repr.hashf == lift_hash_fun ht.hashf /\
     A.is_full_array ht.contents
   )
 
 ```pulse
-fn alloc' (#s:pht_sig_us) (l:pos_us)
+fn alloc' (#k:eqtype) (#v:Type0) (hashf:(k -> US.t)) (l:pos_us)
   requires emp
-  returns ht:ht_t s
-  ensures exists pht. models s ht pht
+  returns ht:ht_t k v
+  ensures exists pht. models ht pht
 {
-  let contents = A.alloc #(cell s.keyt s.valt) Clean l;
-  let ht = mk_ht l contents;
-  let pht = Ghost.hide (mk_init_pht #s l);
+  let contents = A.alloc #(cell k v) Clean l;
+  let ht = mk_ht l hashf contents;
+  let pht = Ghost.hide (mk_init_pht #k #v hashf l);
   rewrite (A.pts_to contents (Seq.create (SZ.v l) Clean))
-    as (A.pts_to ht.contents pht.repr);
-  fold (models s ht pht);
+    as (A.pts_to ht.contents pht.repr.seq);
+  fold (models ht pht);
   ht
 }
 ```
@@ -38,25 +39,26 @@ let perform (#a:Type0) (#b:Type0) (f:  (a -> stt b emp (fun _ -> emp))) (x:a)
   : stt b emp (fun _ -> emp)
   = f x
 
+#push-options "--query_stats --log_queries"
 ```pulse
-fn dealloc' (#s:pht_sig_us) (ht:ht_t s) (l:pos_us) 
-  (destroy_val:destroy_fn_t s.valt)
-  (destroy_key:destroy_fn_t s.keyt)
-  requires exists pht. models s ht pht
+fn dealloc' (#k:eqtype) (#v:Type0) (ht:ht_t k v)
+  (destroy_val:destroy_fn_t v)
+  (destroy_key:destroy_fn_t k)
+  requires exists pht. models ht pht
   ensures emp
 {
   open SZ;
   let mut off = 0sz;
 
-  with pht. assert (models s ht pht);
-  unfold (models s ht pht);
+  with pht. assert (models ht pht);
+  unfold (models ht pht);
 
   while (let voff = !off; (voff <^ ht.sz))
   invariant b. exists (voff:SZ.t). (
-    A.pts_to ht.contents pht.repr **
+    A.pts_to ht.contents pht.repr.seq **
     R.pts_to off voff **
     pure (
-      SZ.v ht.sz == pht.sz /\
+      SZ.v ht.sz == pht.repr.sz /\
       voff <=^ ht.sz /\
       b == (voff <^ ht.sz)
     )
@@ -93,29 +95,29 @@ let sz_add (x y : SZ.t)
     )
     else None
 
-#push-options "--z3rlimit_factor 4 --query_stats"
+#push-options "--z3rlimit_factor 4 --query_stats"// --admit_smt_queries true"
 ```pulse
-fn pulse_lookup_index (#s:pht_sig_us)
-                      (#pht:erased (pht_t (s_to_ps s)))
-                      (ht:ht_t s) (k:s.keyt)
-  requires models s ht pht
-  returns  p:bool & option (s.valt & SZ.t)
-  ensures  models s ht pht ** 
+fn pulse_lookup_index (#kt:eqtype) (#vt:Type0)
+                      (#pht:erased (pht_t kt vt))
+                      (ht:ht_t kt vt) (k:kt)
+  requires models ht pht
+  returns  p:bool & option (vt & SZ.t)
+  ensures  models ht pht ** 
            pure ( fst p ==> (snd p) == PHT.lookup_index_us pht k )
 {
   open SZ;
-  let cidx = s.hashf k %^ ht.sz;
+  let cidx = ht.hashf k %^ ht.sz;
   let mut off = 0sz;
   let mut cont = true;
   let mut err = false;
-  let mut ret = None #(s.valt & SZ.t);
-  unfold (models s ht pht);
+  let mut ret = None #(vt & SZ.t);
+  unfold (models ht pht);
   while (let voff = !off;
          let vcont = !cont;
          let verr = !err; 
          (voff <=^ ht.sz && vcont = true && verr = false)) 
   invariant b. exists (voff:SZ.t) (vcont verr:bool). (
-    A.pts_to ht.contents pht.repr **
+    A.pts_to ht.contents pht.repr.seq **
     R.pts_to off voff **
     R.pts_to cont vcont **
     R.pts_to err verr **
@@ -123,8 +125,8 @@ fn pulse_lookup_index (#s:pht_sig_us)
     pure (
       SZ.v ht.sz == pht_sz pht /\
       voff <=^ ht.sz /\
-      walk_get_idx #(s_to_ps s) #(pht_sz pht) pht.repr (SZ.v cidx) k (SZ.v voff) 
-        == lookup_repr_index #(s_to_ps s) #(pht_sz pht) pht.repr k /\
+      walk_get_idx pht.repr (SZ.v cidx) k (SZ.v voff) 
+        == lookup_repr_index pht.repr k /\
       b == (voff <=^ ht.sz && vcont = true && verr = false)
     ))
   {
@@ -184,7 +186,7 @@ fn pulse_lookup_index (#s:pht_sig_us)
   };
   let verr = !err;
   let o = !ret;
-  fold (models s ht pht);
+  fold (models ht pht);
   if verr
   {
     (false,o)
@@ -198,158 +200,46 @@ fn pulse_lookup_index (#s:pht_sig_us)
 ```
 #pop-options
 ```pulse
-fn lookup' (#s:pht_sig_us)
-           (#pht:erased (pht_t (s_to_ps s)))
-           (ht:ht_t s) (k:s.keyt)
-  requires models s ht pht
-  returns  p:bool & option s.valt
-  ensures  models s ht pht ** 
+fn lookup' (#kt:eqtype) (#vt:Type0)
+           (#pht:erased (pht_t kt vt))
+           (ht:ht_t kt vt) (k:kt)
+  requires models ht pht
+  returns  p:bool & option vt
+  ensures  models ht pht ** 
            pure ( fst p ==> (snd p) == PHT.lookup pht k )
 {
-  let p = pulse_lookup_index #s #pht ht k;
+  let p = pulse_lookup_index #_ #_ #pht ht k;
   if (fst p)
   {
     match (snd p)
     {
       Some p -> { (true, Some (fst p)) }
-      None -> { (true, None #s.valt) }
+      None -> { (true, None #vt) }
     }
   } 
   else
   {
-    (false, None #s.valt)
+    (false, None #vt)
   }
 }
 ```
 let lookup = lookup'
 
-#push-options "--z3rlimit_factor 8 --query_stats"
-open Pulse.Lib.BoundedIntegers
-
-```pulse
-fn insert' (#s:pht_sig_us)
-           (#pht:(p:erased (pht_t (s_to_ps s)){PHT.not_full p.repr}))
-           (ht:ht_t s) (k:s.keyt) (v:s.valt)
-  requires models s ht pht
-  returns b:bool
-  ensures maybe_update b s ht pht (PHT.insert pht k v)
-{
-  let cidx = s.hashf k % ht.sz;
-  // match opt_cidx {
-  // Some cidx -> {
-  assert (pure (SZ.v cidx == SZ.v (s.hashf k) % SZ.v ht.sz));
-  let mut off = 0sz;
-  let mut cont = true;
-  let mut err = false;
-
-  unfold (models s ht pht);
-
-  while (let voff = !off; let vcont = !cont; let verr = !err; (voff <= ht.sz && vcont = true && verr = false)) 
-  invariant b. exists (voff:SZ.t) (vcont verr:bool). (
-    R.pts_to off voff **
-    R.pts_to cont vcont **
-    R.pts_to err verr **
-    A.pts_to ht.contents (if (vcont || verr) then pht.repr else (PHT.insert pht k v).repr) **
-    pure (
-      SZ.v ht.sz == pht_sz pht /\
-      voff <= ht.sz /\
-      strong_all_used_not_by pht.repr (SZ.v cidx) (SZ.v voff) k /\
-      walk pht.repr (SZ.v cidx) k (SZ.v voff) == lookup_repr pht.repr k /\
-      insert_repr_walk #(s_to_ps s) #(pht_sz pht) #pht.spec pht.repr k v (SZ.v voff) (SZ.v cidx) () () 
-        == insert_repr #(s_to_ps s) #(pht_sz pht) #pht.spec pht.repr k v /\
-      b == (voff <= ht.sz && vcont = true && verr = false)
-    ))
-  {
-    let voff = !off;
-    if (voff = ht.sz) {
-      cont := false;
-      assert (A.pts_to ht.contents pht.repr);
-    } else {
-      let opt_sum = cidx `safe_add` voff;
-      match opt_sum {
-      Some sum -> {
-        let idx = sum % ht.sz;
-        let c = (ht.contents).(idx); 
-        match c {
-        Used k' v' -> { 
-          if (k' = k) {
-            assert (A.pts_to ht.contents pht.repr);
-            assert (pure ( SZ.v idx < Seq.length pht.repr));
-            ((ht.contents).(idx) <- (mk_used_cell k v));
-            cont := false;
-            assert (pure (insert_repr #(s_to_ps s) #(pht_sz pht) #pht.spec pht.repr k v `Seq.equal` 
-                          Seq.upd pht.repr (SZ.v idx) (mk_used_cell k v))); 
-          } else {
-            off := voff + 1sz;
-          } 
-        }
-        Clean -> {
-          ((ht.contents).(idx) <- (mk_used_cell k v));
-          cont := false;
-          assert (pure (insert_repr #(s_to_ps s) #(pht_sz pht) #pht.spec pht.repr k v `Seq.equal` 
-                  Seq.upd pht.repr (SZ.v idx) (mk_used_cell k v)));
-        }
-        Zombie -> {
-          fold (models s ht pht);
-          let res = pulse_lookup_index #s #pht ht k;
-          unfold (models s ht pht);
-          if (fst res) {
-            let o = snd res;
-            match o {
-              Some p -> {
-                ((ht.contents).(snd p) <- Zombie);
-                ((ht.contents).(idx) <- (mk_used_cell k v));
-                cont := false;
-                assert (pure (insert_repr #(s_to_ps s) #(pht_sz pht) #pht.spec pht.repr k v `Seq.equal` 
-                              Seq.upd (Seq.upd pht.repr (SZ.v (snd p)) Zombie) (SZ.v idx) (mk_used_cell k v)));
-              }
-              None -> { 
-                ((ht.contents).(idx) <- (mk_used_cell k v)); 
-                cont := false;
-                assert (pure (insert_repr #(s_to_ps s) #(pht_sz pht) #pht.spec pht.repr k v `Seq.equal`
-                              Seq.upd pht.repr (SZ.v idx) (mk_used_cell k v)));
-              }
-          }} else {
-            // ERROR - lookup failed
-            err := true;
-          }
-        }
-      }
-    }
-    None -> {
-      // ERROR - add failed
-      err := true 
-    }}}
-  };
-  let verr = !err;
-  if verr {
-    fold (models s ht pht);
-    fold (maybe_update false s ht pht (PHT.insert pht k v));
-    false
-  } else {
-    fold (models s ht (PHT.insert pht k v));
-    fold (maybe_update true s ht pht (PHT.insert pht k v));
-    true
-  }
-  // }
-
-  // None -> {
-  //   fold (maybe_update false s ht pht (PHT.insert pht k v));
-  //   false
-  // }}
-}
-```
+// #push-options "--z3rlimit_factor 8 --query_stats --log_queries"
+// #restart-solver
+// open Pulse.Lib.BoundedIntegers
 
 // ```pulse
 // fn insert' (#s:pht_sig_us)
 //            (#pht:(p:erased (pht_t (s_to_ps s)){PHT.not_full p.repr}))
-//            (ht:ht_t s) (k:s.keyt) (value:s.valt)
+//            (ht:ht_t s) (k:s.keyt) (v:s.valt)
 //   requires models s ht pht
 //   returns b:bool
-//   ensures maybe_update b s ht pht (PHT.insert pht k value)
+//   ensures maybe_update b s ht pht (PHT.insert pht k v)
 // {
-//   // open SZ;
 //   let cidx = SZ.(s.hashf k %^ ht.sz);
+//   // match opt_cidx {
+//   // Some cidx -> {
 //   assert (pure (SZ.v cidx == SZ.v (s.hashf k) % SZ.v ht.sz));
 //   let mut off = 0sz;
 //   let mut cont = true;
@@ -357,23 +247,276 @@ fn insert' (#s:pht_sig_us)
 
 //   unfold (models s ht pht);
 
-//   while (let voff = !off;
-//          let vcont = !cont;
-//          let verr = !err; 
-//          (SZ.(voff <=^ ht.sz) && vcont = true && verr = false)) 
+//   while (let voff = !off; let vcont = !cont; let verr = !err; (SZ.(voff <=^ ht.sz) && vcont = true && verr = false)) 
 //   invariant b. exists (voff:SZ.t) (vcont verr:bool). (
 //     R.pts_to off voff **
 //     R.pts_to cont vcont **
 //     R.pts_to err verr **
-//     A.pts_to ht.contents (if (vcont || verr) then pht.repr else (PHT.insert pht k value).repr) **
+//     A.pts_to ht.contents (if (vcont || verr) then pht.repr else (PHT.insert pht k v).repr) **
 //     pure (
 //       SZ.v ht.sz == pht_sz pht /\
 //       SZ.(voff <=^ ht.sz) /\
 //       strong_all_used_not_by pht.repr (SZ.v cidx) (SZ.v voff) k /\
 //       walk pht.repr (SZ.v cidx) k (SZ.v voff) == lookup_repr pht.repr k /\
-//       insert_repr_walk #(s_to_ps s) #(pht_sz pht) #pht.spec pht.repr k value (SZ.v voff) (SZ.v cidx) () () 
-//         == insert_repr #(s_to_ps s) #(pht_sz pht) #pht.spec pht.repr k value /\
+//       insert_repr_walk #(s_to_ps s) #(pht_sz pht) #pht.spec pht.repr k v (SZ.v voff) (SZ.v cidx) () () 
+//         == insert_repr #(s_to_ps s) #(pht_sz pht) #pht.spec pht.repr k v /\
 //       b == (SZ.(voff <=^ ht.sz) && vcont = true && verr = false)
+//     ))
+//   {
+//     let voff = !off;
+//     if (voff = ht.sz) {
+//       cont := false;
+//       assert (A.pts_to ht.contents pht.repr);
+//     } else {
+//       let opt_sum = cidx `sz_add` voff;
+//       match opt_sum {
+//       Some sum -> {
+//         let idx = sum % ht.sz;
+//         let c = (ht.contents).(idx); 
+//         match c {
+//         Used k' v' -> { 
+//           if (k' = k) {
+//             assert (A.pts_to ht.contents pht.repr);
+//             assert (pure ( SZ.v idx < Seq.length pht.repr));
+//             ((ht.contents).(idx) <- (mk_used_cell k v));
+//             cont := false;
+//             assert (pure (insert_repr #(s_to_ps s) #(pht_sz pht) #pht.spec pht.repr k v `Seq.equal` 
+//                           Seq.upd pht.repr (SZ.v idx) (mk_used_cell k v))); 
+//           } else {
+//             off := voff + 1sz;
+//           } 
+//         }
+//         Clean -> {
+//           ((ht.contents).(idx) <- (mk_used_cell k v));
+//           cont := false;
+//           assert (pure (insert_repr #(s_to_ps s) #(pht_sz pht) #pht.spec pht.repr k v `Seq.equal` 
+//                   Seq.upd pht.repr (SZ.v idx) (mk_used_cell k v)));
+//         }
+//         Zombie -> {
+//           fold (models s ht pht);
+//           let res = pulse_lookup_index #s #pht ht k;
+//           unfold (models s ht pht);
+//           if (fst res) {
+//             let o = snd res;
+//             match o {
+//               Some p -> {
+//                 ((ht.contents).(snd p) <- Zombie);
+//                 ((ht.contents).(idx) <- (mk_used_cell k v));
+//                 cont := false;
+//                 assert (pure (insert_repr #(s_to_ps s) #(pht_sz pht) #pht.spec pht.repr k v `Seq.equal` 
+//                               Seq.upd (Seq.upd pht.repr (SZ.v (snd p)) Zombie) (SZ.v idx) (mk_used_cell k v)));
+//               }
+//               None -> { 
+//                 ((ht.contents).(idx) <- (mk_used_cell k v)); 
+//                 cont := false;
+//                 assert (pure (insert_repr #(s_to_ps s) #(pht_sz pht) #pht.spec pht.repr k v `Seq.equal`
+//                               Seq.upd pht.repr (SZ.v idx) (mk_used_cell k v)));
+//               }
+//           }} else {
+//             // ERROR - lookup failed
+//             err := true;
+//           }
+//         }
+//       }
+//     }
+//     None -> {
+//       // ERROR - add failed
+//       err := true 
+//     }}}
+//   };
+//   let verr = !err;
+//   if verr {
+//     fold (models s ht pht);
+//     fold (maybe_update false s ht pht (PHT.insert pht k v));
+//     false
+//   } else {
+//     fold (models s ht (PHT.insert pht k v));
+//     fold (maybe_update true s ht pht (PHT.insert pht k v));
+//     true
+//   }
+//   // }
+
+//   // None -> {
+//   //   fold (maybe_update false s ht pht (PHT.insert pht k v));
+//   //   false
+//   // }}
+// }
+// ```
+
+// // ```pulse
+// // fn insert' (#s:pht_sig_us)
+// //            (#pht:(p:erased (pht_t (s_to_ps s)){PHT.not_full p.repr}))
+// //            (ht:ht_t s) (k:s.keyt) (value:s.valt)
+// //   requires models s ht pht
+// //   returns b:bool
+// //   ensures maybe_update b s ht pht (PHT.insert pht k value)
+// // {
+// //   // open SZ;
+// //   let cidx = SZ.(s.hashf k %^ ht.sz);
+// //   assert (pure (SZ.v cidx == SZ.v (s.hashf k) % SZ.v ht.sz));
+// //   let mut off = 0sz;
+// //   let mut cont = true;
+// //   let mut err = false;
+
+// //   unfold (models s ht pht);
+
+// //   while (let voff = !off;
+// //          let vcont = !cont;
+// //          let verr = !err; 
+// //          (SZ.(voff <=^ ht.sz) && vcont = true && verr = false)) 
+// //   invariant b. exists (voff:SZ.t) (vcont verr:bool). (
+// //     R.pts_to off voff **
+// //     R.pts_to cont vcont **
+// //     R.pts_to err verr **
+// //     A.pts_to ht.contents (if (vcont || verr) then pht.repr else (PHT.insert pht k value).repr) **
+// //     pure (
+// //       SZ.v ht.sz == pht_sz pht /\
+// //       SZ.(voff <=^ ht.sz) /\
+// //       strong_all_used_not_by pht.repr (SZ.v cidx) (SZ.v voff) k /\
+// //       walk pht.repr (SZ.v cidx) k (SZ.v voff) == lookup_repr pht.repr k /\
+// //       insert_repr_walk #(s_to_ps s) #(pht_sz pht) #pht.spec pht.repr k value (SZ.v voff) (SZ.v cidx) () () 
+// //         == insert_repr #(s_to_ps s) #(pht_sz pht) #pht.spec pht.repr k value /\
+// //       b == (SZ.(voff <=^ ht.sz) && vcont = true && verr = false)
+// //     ))
+// //   {
+// //     let voff = !off;
+// //     if (voff = ht.sz)
+// //     {
+// //       cont := false;
+// //       assert (A.pts_to ht.contents pht.repr);
+// //     }
+// //     else
+// //     {
+// //       let opt_sum = cidx `sz_add` voff;
+// //       match opt_sum
+// //       {
+// //         Some sum ->
+// //         {
+// //           let idx = SZ.(sum %^ ht.sz);
+// //           let c = ht.contents.(idx); 
+// //           match c
+// //           {
+// //             Used k' v' ->
+// //             { 
+// //                admit()
+// //       //         if (k' = k)
+// //       //         {
+// //       //           assert (A.pts_to ht.contents pht.repr);
+// //       //           assert (pure ( SZ.v idx < Seq.length pht.repr));
+// //       //           ht.contents.(idx) <- (mk_used_cell k value);
+// //       //           cont := false;
+// //       //           assert (pure (insert_repr #(s_to_ps s) #(pht_sz pht) #pht.spec pht.repr k value `Seq.equal` 
+// //       //                         Seq.upd pht.repr (SZ.v idx) (mk_used_cell k value))); 
+// //       //         }
+// //       //         else
+// //       //         {
+// //       //           off := SZ.(voff +^ 1sz);
+// //       //         } 
+// //             }
+// //             Clean ->
+// //             {
+// //               ht.contents.(idx) <- (mk_used_cell k value);
+// //               cont := false;
+// //               assert (pure (insert_repr #(s_to_ps s) #(pht_sz pht) #pht.spec pht.repr k value `Seq.equal` 
+// //                       Seq.upd pht.repr (SZ.v idx) (mk_used_cell k value)));
+// //             }
+// //             Zombie ->
+// //             {
+// //                  admit()
+// //       //         fold (models s ht pht);
+// //       //         let res = pulse_lookup_index #s #pht ht k;
+// //       //         unfold (models s ht pht);
+// //       //         if (fst res)
+// //       //         {
+// //       //           let o = snd res;
+// //       //           match o
+// //       //           {
+// //       //             Some p ->
+// //       //             {
+// //       //               ht.contents.(snd p) <- Zombie;
+// //       //               ht.contents.(idx) <- (mk_used_cell k value);
+// //       //               cont := false;
+// //       //               assert (pure (insert_repr #(s_to_ps s) #(pht_sz pht) #pht.spec pht.repr k value `Seq.equal` 
+// //       //                             Seq.upd (Seq.upd pht.repr (SZ.v (snd p)) Zombie) (SZ.v idx) (mk_used_cell k value)));
+// //       //             }
+// //       //             None ->
+// //       //             { 
+// //       //               ht.contents.(idx) <- (mk_used_cell k value); 
+// //       //               cont := false;
+// //       //               assert (pure (insert_repr #(s_to_ps s) #(pht_sz pht) #pht.spec pht.repr k value `Seq.equal`
+// //       //                             Seq.upd pht.repr (SZ.v idx) (mk_used_cell k value)));
+// //       //             }
+// //       //           }
+// //       //         } 
+// //       //         else
+// //       //         {
+// //       //           // ERROR - lookup failed
+// //       //           err := true;
+// //       //         }
+// //             }
+// //           }
+// //         }
+// //         None ->
+// //         {
+// //           // ERROR - add failed
+// //           err := true 
+// //         }
+// //       }
+// //     }
+// //   };
+// //   let verr = !err;
+// //   if verr
+// //   {
+// //     fold (models s ht pht);
+// //     fold (maybe_update false s ht pht (PHT.insert pht k value));
+// //     false
+// //   }
+// //   else
+// //   {
+// //     fold (models s ht (PHT.insert pht k value));
+// //     fold (maybe_update true s ht pht (PHT.insert pht k value));
+// //     true
+// //   }
+// // }
+// // ```
+// #pop-options
+
+// let insert = insert'
+
+// #push-options "--z3rlimit_factor 4 --query_stats"
+// #restart-solver
+
+// ```pulse
+// fn delete' (#s:pht_sig_us)
+//            (#pht:erased (pht_t (s_to_ps s)))
+//            (ht:ht_t s) (k:s.keyt)
+//   requires models s ht pht
+//   returns b:bool
+//   ensures maybe_update b s ht pht (PHT.delete pht k)
+// {
+//   let cidx = s.hashf k % ht.sz;
+//   let mut off = 0sz;
+//   let mut cont = true;
+//   let mut err = false;
+
+//   unfold (models s ht pht);
+//   while (let voff = !off;
+//          let vcont = !cont;
+//          let verr = !err; 
+//          (voff <= ht.sz && vcont = true && verr = false))
+//   invariant b. exists (voff:SZ.t) (vcont verr:bool). (
+//     R.pts_to off voff **
+//     R.pts_to cont vcont **
+//     R.pts_to err verr **
+//     A.pts_to ht.contents (if (vcont || verr) then pht.repr else (PHT.delete pht k).repr) **
+//     pure (
+//       SZ.v ht.sz == pht_sz pht /\
+//       voff <= ht.sz /\
+//       all_used_not_by pht.repr (SZ.v cidx) (SZ.v voff) k /\
+//       walk pht.repr (SZ.v cidx) k (SZ.v voff) == lookup_repr pht.repr k /\
+//       delete_repr_walk #(s_to_ps s) #(pht_sz pht) #pht.spec pht.repr k (SZ.v voff) (SZ.v cidx) () () 
+//         == delete_repr #(s_to_ps s) #(pht_sz pht) #pht.spec pht.repr k /\
+//       b == (voff <= ht.sz && vcont = true && verr = false)
 //     ))
 //   {
 //     let voff = !off;
@@ -384,79 +527,45 @@ fn insert' (#s:pht_sig_us)
 //     }
 //     else
 //     {
-//       let opt_sum = cidx `sz_add` voff;
+//       let opt_sum = cidx `safe_add` voff;
 //       match opt_sum
 //       {
 //         Some sum ->
 //         {
-//           let idx = SZ.(sum %^ ht.sz);
+//           let idx = sum % ht.sz;
 //           let c = ht.contents.(idx); 
 //           match c
 //           {
 //             Used k' v' ->
 //             { 
-//                admit()
-//       //         if (k' = k)
-//       //         {
-//       //           assert (A.pts_to ht.contents pht.repr);
-//       //           assert (pure ( SZ.v idx < Seq.length pht.repr));
-//       //           ht.contents.(idx) <- (mk_used_cell k value);
-//       //           cont := false;
-//       //           assert (pure (insert_repr #(s_to_ps s) #(pht_sz pht) #pht.spec pht.repr k value `Seq.equal` 
-//       //                         Seq.upd pht.repr (SZ.v idx) (mk_used_cell k value))); 
-//       //         }
-//       //         else
-//       //         {
-//       //           off := SZ.(voff +^ 1sz);
-//       //         } 
+//               if (k' = k)
+//               {
+//                 ht.contents.(idx) <- Zombie;
+//                 cont := false;
+//                 assert (pure (pht.repr @@ SZ.v idx == Used k v'));
+//                 assert (pure (Seq.upd pht.repr (SZ.v idx) Zombie 
+//                   `Seq.equal` (PHT.delete pht k).repr));
+//               }
+//               else
+//               {
+//                 off := voff + 1sz;
+//               } 
 //             }
 //             Clean ->
 //             {
-//               ht.contents.(idx) <- (mk_used_cell k value);
 //               cont := false;
-//               assert (pure (insert_repr #(s_to_ps s) #(pht_sz pht) #pht.spec pht.repr k value `Seq.equal` 
-//                       Seq.upd pht.repr (SZ.v idx) (mk_used_cell k value)));
+//               assert (pure (pht.repr == (PHT.delete pht k).repr));
 //             }
 //             Zombie ->
 //             {
-//                  admit()
-//       //         fold (models s ht pht);
-//       //         let res = pulse_lookup_index #s #pht ht k;
-//       //         unfold (models s ht pht);
-//       //         if (fst res)
-//       //         {
-//       //           let o = snd res;
-//       //           match o
-//       //           {
-//       //             Some p ->
-//       //             {
-//       //               ht.contents.(snd p) <- Zombie;
-//       //               ht.contents.(idx) <- (mk_used_cell k value);
-//       //               cont := false;
-//       //               assert (pure (insert_repr #(s_to_ps s) #(pht_sz pht) #pht.spec pht.repr k value `Seq.equal` 
-//       //                             Seq.upd (Seq.upd pht.repr (SZ.v (snd p)) Zombie) (SZ.v idx) (mk_used_cell k value)));
-//       //             }
-//       //             None ->
-//       //             { 
-//       //               ht.contents.(idx) <- (mk_used_cell k value); 
-//       //               cont := false;
-//       //               assert (pure (insert_repr #(s_to_ps s) #(pht_sz pht) #pht.spec pht.repr k value `Seq.equal`
-//       //                             Seq.upd pht.repr (SZ.v idx) (mk_used_cell k value)));
-//       //             }
-//       //           }
-//       //         } 
-//       //         else
-//       //         {
-//       //           // ERROR - lookup failed
-//       //           err := true;
-//       //         }
+//               off := voff + 1sz;
 //             }
 //           }
 //         }
 //         None ->
 //         {
 //           // ERROR - add failed
-//           err := true 
+//           err := false 
 //         }
 //       }
 //     }
@@ -465,167 +574,61 @@ fn insert' (#s:pht_sig_us)
 //   if verr
 //   {
 //     fold (models s ht pht);
-//     fold (maybe_update false s ht pht (PHT.insert pht k value));
+//     fold (maybe_update false s ht pht (PHT.delete pht k));
 //     false
 //   }
 //   else
 //   {
-//     fold (models s ht (PHT.insert pht k value));
-//     fold (maybe_update true s ht pht (PHT.insert pht k value));
+//     fold (models s ht (PHT.delete pht k));
+//     fold (maybe_update true s ht pht (PHT.delete pht k));
 //     true
 //   }
 // }
 // ```
-#pop-options
-
-let insert = insert'
-
-#push-options "--z3rlimit_factor 4 --query_stats"
-#restart-solver
-
-```pulse
-fn delete' (#s:pht_sig_us)
-           (#pht:erased (pht_t (s_to_ps s)))
-           (ht:ht_t s) (k:s.keyt)
-  requires models s ht pht
-  returns b:bool
-  ensures maybe_update b s ht pht (PHT.delete pht k)
-{
-  let cidx = s.hashf k % ht.sz;
-  let mut off = 0sz;
-  let mut cont = true;
-  let mut err = false;
-
-  unfold (models s ht pht);
-  while (let voff = !off;
-         let vcont = !cont;
-         let verr = !err; 
-         (voff <= ht.sz && vcont = true && verr = false))
-  invariant b. exists (voff:SZ.t) (vcont verr:bool). (
-    R.pts_to off voff **
-    R.pts_to cont vcont **
-    R.pts_to err verr **
-    A.pts_to ht.contents (if (vcont || verr) then pht.repr else (PHT.delete pht k).repr) **
-    pure (
-      SZ.v ht.sz == pht_sz pht /\
-      voff <= ht.sz /\
-      all_used_not_by pht.repr (SZ.v cidx) (SZ.v voff) k /\
-      walk pht.repr (SZ.v cidx) k (SZ.v voff) == lookup_repr pht.repr k /\
-      delete_repr_walk #(s_to_ps s) #(pht_sz pht) #pht.spec pht.repr k (SZ.v voff) (SZ.v cidx) () () 
-        == delete_repr #(s_to_ps s) #(pht_sz pht) #pht.spec pht.repr k /\
-      b == (voff <= ht.sz && vcont = true && verr = false)
-    ))
-  {
-    let voff = !off;
-    if (voff = ht.sz)
-    {
-      cont := false;
-      assert (A.pts_to ht.contents pht.repr);
-    }
-    else
-    {
-      let opt_sum = cidx `safe_add` voff;
-      match opt_sum
-      {
-        Some sum ->
-        {
-          let idx = sum % ht.sz;
-          let c = ht.contents.(idx); 
-          match c
-          {
-            Used k' v' ->
-            { 
-              if (k' = k)
-              {
-                ht.contents.(idx) <- Zombie;
-                cont := false;
-                assert (pure (pht.repr @@ SZ.v idx == Used k v'));
-                assert (pure (Seq.upd pht.repr (SZ.v idx) Zombie 
-                  `Seq.equal` (PHT.delete pht k).repr));
-              }
-              else
-              {
-                off := voff + 1sz;
-              } 
-            }
-            Clean ->
-            {
-              cont := false;
-              assert (pure (pht.repr == (PHT.delete pht k).repr));
-            }
-            Zombie ->
-            {
-              off := voff + 1sz;
-            }
-          }
-        }
-        None ->
-        {
-          // ERROR - add failed
-          err := false 
-        }
-      }
-    }
-  };
-  let verr = !err;
-  if verr
-  {
-    fold (models s ht pht);
-    fold (maybe_update false s ht pht (PHT.delete pht k));
-    false
-  }
-  else
-  {
-    fold (models s ht (PHT.delete pht k));
-    fold (maybe_update true s ht pht (PHT.delete pht k));
-    true
-  }
-}
-```
-let delete = delete'
+// let delete = delete'
 
 
-```pulse
-fn not_full' (#s:pht_sig_us) (#pht:erased (pht_t (s_to_ps s))) (ht:ht_t s)
-  requires models s ht pht
-  returns b:bool
-  ensures models s ht pht ** 
-          pure (b ==> PHT.not_full #(s_to_ps s) #(pht_sz pht) pht.repr)
-{
-  let mut i = 0sz;
-  unfold (models s ht pht);
+// ```pulse
+// fn not_full' (#s:pht_sig_us) (#pht:erased (pht_t (s_to_ps s))) (ht:ht_t s)
+//   requires models s ht pht
+//   returns b:bool
+//   ensures models s ht pht ** 
+//           pure (b ==> PHT.not_full #(s_to_ps s) #(pht_sz pht) pht.repr)
+// {
+//   let mut i = 0sz;
+//   unfold (models s ht pht);
 
-  while
-  (
-    let vi = !i;  
-    if (vi < ht.sz) 
-    { 
-      let c = ht.contents.(vi); 
-      (Used? c) 
-    }
-    else 
-    { 
-      false
-    }
-  )
-  invariant b. exists (vi:SZ.t). (
-    A.pts_to ht.contents pht.repr **
-    R.pts_to i vi **
-    pure (
-      SZ.v ht.sz == pht_sz pht /\
-      vi <= ht.sz /\
-      (b == (vi < ht.sz && Used? (pht.repr @@ (SZ.v vi)))) /\
-      (forall (i:nat). i < SZ.v vi ==> Used? (pht.repr @@ i))
-    )
-  )
-  {
-    let vi = !i;
-    i := vi + 1sz;
-  };
-  let vi = !i;
-  let res = vi < ht.sz;
-  fold (models s ht pht);  
-  res
-}
-```
-let not_full = not_full'
+//   while
+//   (
+//     let vi = !i;  
+//     if (vi < ht.sz) 
+//     { 
+//       let c = ht.contents.(vi); 
+//       (Used? c) 
+//     }
+//     else 
+//     { 
+//       false
+//     }
+//   )
+//   invariant b. exists (vi:SZ.t). (
+//     A.pts_to ht.contents pht.repr **
+//     R.pts_to i vi **
+//     pure (
+//       SZ.v ht.sz == pht_sz pht /\
+//       vi <= ht.sz /\
+//       (b == (vi < ht.sz && Used? (pht.repr @@ (SZ.v vi)))) /\
+//       (forall (i:nat). i < SZ.v vi ==> Used? (pht.repr @@ i))
+//     )
+//   )
+//   {
+//     let vi = !i;
+//     i := vi + 1sz;
+//   };
+//   let vi = !i;
+//   let res = vi < ht.sz;
+//   fold (models s ht pht);  
+//   res
+// }
+// ```
+// let not_full = not_full'
